assembly/Machine.v
@@ -1,10 +1,9 @@
-Require Import Utf8.
-
 Require Import Equations.Equations.
 
 Require Import Assembly.Mon.
 Require Import Assembly.Bits.
 Require Import Assembly.Dec.
+Require Import Assembly.Convenience.
 Require Import Assembly.Operations.
 Require Assembly.OpCodes.
 
@@ -12,11 +11,13 @@ Require Assembly.OpCodes.
 Context
   (memStart: nat) (* TODO: Use B64 instead? *)
   (memSize: nat)
-  (inputImages : list (Image B8)).
-
-Notation as_bool x := (if x then true else false).
+  (inputImages : list (Image B8))
+  (State: Type).
 
 Module Export MT <: machine_type.
+  Definition State := State.
+  Definition M := EST State.
+  Definition H_mon := est_smonad State.
   Definition Addr := B64.
   Definition H_eqdec := (ltac:(typeclasses eauto) : EqDec B64).
   Definition available := fun (a: B64) => as_bool (decision (memStart <= a /\ a < memStart + memSize)).
@@ -34,258 +35,300 @@ End MT.
 
 Include core_module MT.
 
+Identity Coercion id_Addr : Addr >-> B64.
+Identity Coercion id_Cell : Cell >-> B8.
+Identity Coercion id_InputColor : InputColor >-> B8.
+Identity Coercion id_Char : Char >-> B32.
+Identity Coercion id_Byte : Byte >-> B8.
+Identity Coercion id_Sample : Sample >-> B16.
+
 Definition nextN (n: nat) : M nat :=
   let* bytes := next n in
-  ret (fromLittleEndian (bytes : Vector.t _ _)).
+  ret (fromLittleEndian bytes).
 
 Definition push64 (z: Z) : M unit :=
   pushMany (toLittleEndian 8 z).
 
 Definition popN : M nat :=
   let* bytes := popMany 8 in
-  ret (fromLittleEndian (bytes : Vector.t _ _)).
+  ret (fromLittleEndian bytes).
 
 Definition pop64 : M B64 :=
   let* x := popN in
-  ret (toB64 (x: nat)).
+  ret (toB64 x).
 
 Definition loadN (n: nat) (a: Z) : M nat :=
   let* bytes := loadMany n (toB64 a) in
-  ret (fromLittleEndian (bytes : Vector.t _ _)).
+  ret (fromLittleEndian bytes).
 
 Definition storeZ (n: nat) (a: Z) (x: Z) : M unit :=
   storeMany (toB64 a) (map Some (toLittleEndian n x)).
 
 Import OpCodes.
 
-Definition oneStep : M bool :=
-  let exit := ret false : M bool in
-  let continue := ret true : M bool in
-  let error := err : M bool in
+(* Without [noind] solving obligations seems to go on forever.
+   Alas, this still generated 257 equations... *)
+Equations(noind) oneStep' (op: nat) : M unit :=
+  oneStep' NOP := ret tt;
 
-  let* opcode := nextN 1 in
-  match opcode with
-  | EXIT => exit
-  | NOP => continue
+  oneStep' JUMP :=
+    let* a := popN in
+    put' PC (toB64 a);
 
-  | JUMP =>
-      let* a := popN in
-      put' PC (toB64 (a: nat));;
-      continue
-
-  | JUMP_ZERO =>
+  oneStep' JUMP_ZERO :=
       let* o := nextN 1 in
       let* x := popN in
       (if (decision (x = 0))
        then
          let* pc := get' PC in
-         put' PC (offset (signed (toB8 (o: nat))) pc)
+         put' PC (offset (signed (toB8 o)) pc)
        else
-         ret tt);;
-      continue
+         ret tt);
 
-  | SET_SP =>
+  oneStep' SET_SP :=
       let* a := pop64 in
-      put' SP a;;
-      continue
+      put' SP a;
 
-  | GET_PC =>
+  oneStep' GET_PC =>
       let* a := get' PC in
-      push64 (a: B64);;
-      continue
+      push64 a;
 
-  | GET_SP =>
+  oneStep' GET_SP :=
       let* a := get' SP in
-      push64 (a: B64);;
-      continue
+      push64 a;
 
-  | PUSH0 =>
-      push64 0;;
-      continue
+  oneStep' PUSH0 :=
+      push64 0;
 
-  | PUSH1 =>
+  oneStep' PUSH1 :=
       let* x := nextN 1 in
-      push64 (x: nat);;
-      continue
+      push64 x;
 
-  | PUSH2 =>
+  oneStep' PUSH2 :=
       let* x := nextN 2 in
-      push64 (x: nat);;
-      continue
+      push64 x;
 
-  | PUSH4 =>
+  oneStep' PUSH4 :=
       let* x := nextN 4 in
-      push64 (x: nat);;
-      continue
+      push64 x;
 
-  | PUSH8 =>
+  oneStep' PUSH8 :=
       let* x := nextN 8 in
-      push64 (x: nat);;
-      continue
+      push64 x;
 
-  | SIGX1 =>
+  oneStep' SIGX1 :=
       let* x := popN in
-      push64 (signed (toB8 (x: nat)));;
-      continue
+      push64 (signed (toB8 x));
 
-  | SIGX2 =>
+  oneStep' SIGX2 :=
       let* x := popN in
-      push64 (signed (toB16 (x: nat)));;
-      continue
+      push64 (signed (toB16 x));
 
-  | SIGX4 =>
+  oneStep' SIGX4 :=
       let* x := popN in
-      push64 (signed (toB32 (x : nat)));;
-      continue
+      push64 (signed (toB32 x));
 
-  | LOAD1 =>
+  oneStep' LOAD1 :=
       let* a := popN in
-      let* x := loadN 1 (a: nat) in
-      push64 (x: nat);;
-      continue
+      let* x := loadN 1 a in
+      push64 x;
 
-  | LOAD2 =>
+  oneStep' LOAD2 :=
       let* a := popN in
-      let* x := loadN 2 (a: nat) in
-      push64 (x: nat);;
-      continue
+      let* x := loadN 2 a in
+      push64 x;
 
-  | LOAD4 =>
+  oneStep' LOAD4 :=
       let* a := popN in
-      let* x := loadN 4 (a: nat) in
-      push64 (x: nat);;
-      continue
+      let* x := loadN 4 a in
+      push64 x;
 
-  | LOAD8 =>
+  oneStep' LOAD8 :=
       let* a := popN in
-      let* x := loadN 8 (a: nat) in
-      push64 (x: nat);;
-      continue
+      let* x := loadN 8 a in
+      push64 x;
 
-  | STORE1 =>
+  oneStep' STORE1 :=
       let* a := popN in
       let* x := popN in
-      storeZ 1 (a: nat) (x: nat);;
-      continue
+      storeZ 1 a x;
 
-  | STORE2 =>
+  oneStep' STORE2 :=
       let* a := popN in
       let* x := popN in
-      storeZ 2 (a: nat) (x: nat);;
-      continue
+      storeZ 2 a x;
 
-  | STORE4 =>
+  oneStep' STORE4 :=
       let* a := popN in
       let* x := popN in
-      storeZ 4 (a: nat) (x: nat);;
-      continue
+      storeZ 4 a x;
 
-  | STORE8 =>
+  oneStep' STORE8 :=
       let* a := popN in
       let* x := popN in
-      storeZ 8 (a: nat) (x: nat);;
-      continue
+      storeZ 8 a x;
 
-  | ADD =>
+  oneStep' ADD :=
       let* x := popN in
       let* y := popN in
-      push64 ((x:nat) + (y:nat));;
-      continue
+      push64 (x + (y:nat));
 
-  | MULT =>
+  oneStep' MULT :=
       let* x := popN in
       let* y := popN in
-      push64 ((x:nat) * (y:nat));;
-      continue
+      push64 (x * (y:nat));
 
-  | DIV =>
+  oneStep' DIV :=
       let* x := popN in
       let* y := popN in
-      push64 (if decision (x=0) then 0 else (y:nat) / x);;
-      continue
+      push64 (if decision (x=0) then 0 else (y:nat) / x);
 
-  | REM =>
+  oneStep' REM :=
       let* x := popN in
       let* y := popN in
-      push64 (if decision (x=0) then 0 else (y:nat) mod x);;
-      continue
+      push64 (if decision (x=0) then 0 else (y:nat) mod x);
 
-  | LT =>
+  oneStep' LT :=
       let* x := popN in
       let* y := popN in
-      push64 (if decision (y < x) then -1 else 0);;
-      continue
+      push64 (if decision (y < x) then -1 else 0);
 
-  | AND =>
+  oneStep' AND :=
       let* x := pop64 in
       let* y := pop64 in
-      push64 (Vector.map2 andb x y : B64);;
-      continue
+      push64 (Vector.map2 andb x y : B64);
 
-  | OR =>
+  oneStep' OR :=
       let* x := pop64 in
       let* y := pop64 in
-      push64 (Vector.map2 orb x y : B64);;
-      continue
+      push64 (Vector.map2 orb x y : B64);
 
-  | NOT =>
+  oneStep' NOT :=
       let* x := pop64 in
-      push64 (Vector.map negb x : B64);;
-      continue
+      push64 (Vector.map negb x : B64);
 
-  | XOR =>
+  oneStep' XOR :=
       let* x := pop64 in
       let* y := pop64 in
-      push64 (Vector.map2 xorb x y : B64);;
-      continue
+      push64 (Vector.map2 xorb x y : B64);
 
-  (* *** *)
-
-  | READ_FRAME =>
+  oneStep' READ_FRAME :=
       let* i := popN in
       let* pair := readFrame (i: nat) in
-      push64 (fst pair : nat);;
-      push64 (snd pair : nat);;
-      continue
+      push64 (fst pair);;
+      push64 (snd pair);
 
-  | READ_PIXEL =>
+  oneStep' READ_PIXEL :=
       let* y := popN in
       let* x := popN in
-      let* c := readPixel (x:nat) (y:nat) in
-      push64 (c:B8);;
-      continue
+      let* c := readPixel x y in
+      push64 c;
 
-  | NEW_FRAME =>
+  oneStep' NEW_FRAME :=
       let* r := popN in
       let* h := popN in
       let* w := popN in
-      newFrame (w:nat) (h:nat) (r:nat);;
-      continue
+      newFrame w h r;
 
-  | SET_PIXEL =>
+  oneStep' SET_PIXEL :=
       let* b := pop64 in
       let* g := pop64 in
       let* r := pop64 in
       let* y := popN in
       let* x := popN in
-      setPixel (x:nat) (y:nat) (r:B64, g:B64, b:B64);;
-      continue
+      setPixel x y (r, g, b);
 
-  | ADD_SAMPLE =>
+  oneStep' ADD_SAMPLE :=
       let* r := popN in
       let* l := popN in
-      addSample (toB16 (l:nat)) (toB16 (r:nat));;
-      continue
+      addSample (toB16 l) (toB16 r);
 
-  | PUT_CHAR =>
+  oneStep' PUT_CHAR :=
       let* c := popN in
-      putChar (toB32 (c:nat));;
-      continue
+      putChar (toB32 c);
 
-  | PUT_BYTE =>
+  oneStep' PUT_BYTE :=
       let* b := popN in
-      putByte (toB8 (b:nat));;
-      continue
+      putByte (toB8 b);
 
-  | _ => error
+  oneStep' _ := err.
+
+Definition oneStep : M bool :=
+  let* op := nextN 1 in
+  match op with
+  | EXIT => ret false
+  | _ => oneStep' op;; ret true
   end.
+
+(** The machine will reach [doneState]
+    if we start the machine in the given state
+    and run as long as [while] does not fail. *)
+
+Inductive OkFrom (while: M unit) (post: State -> Prop) : State -> Prop :=
+| Done s : not (while s) -> post s -> OkFrom while post s
+| More s (_: while s) s': oneStep s = Some (s', true)
+                          -> OkFrom while post s'
+                          -> OkFrom while post s.
+
+(** Using elements of [M unit] is a quick and dirty way to express the
+    decidable predicates on [State], where side-effects other than [err]
+    are essentially ignored. *)
+
+Definition unconditionally : M unit := ret tt.
+
+Definition opsAtPc (ops: list B8) : M unit :=
+  let* pc := get' PC in
+  let* bytes := loadMany (length ops) pc in
+  assert* ops = bytes in
+  unconditionally.
+
+Definition pcInRegion (n: nat) (s: State) : M unit :=
+  match get' PC s with
+  | None => err (* This will never happen. *)
+  | Some (_, start) =>
+      let* pc := get' PC in
+      let i := Z.to_nat ((pc - start) mod 2^64)%Z in
+      assert* i < n in
+      unconditionally
+  end.
+
+Class Spec (ops: list nat) :=
+{
+  precondition: M unit;
+  postcondition: State -> State -> Prop;
+  witness s : opsAtPc (map (fun (op:nat) => toB8 op) ops) s
+              -> precondition s
+              -> OkFrom (pcInRegion (length ops) s) (postcondition s) s;
+}.
+
+#[refine]
+Instance trivial_spec : Spec [] :=
+{
+  precondition := unconditionally;
+  postcondition := eq;
+  witness s _ _ := Done _ _ s _ _;
+}.
+Proof.
+  all: tauto.
+Qed.
+
+#[refine]
+Instance nop_spec : Spec [NOP] :=
+{
+  precondition := unconditionally;
+  postcondition s := eq (update (Proj:=PC) s (offset 1 (proj (Proj:=PC) s)));
+  witness s _ _ := _;
+}.
+Proof.
+  match goal with
+    [|- OkFrom ?x (eq ?y) s] => set (w:=x); set (s':=y) end.
+  apply (More w unconditionally s _ s').
+
+
+  set (s' := @update State Addr PC s (offset (Zpos xH) (@proj State Addr PC s))).
+
+  set (s' := update s (Proj:=PC) (offset 1 (proj s))).
+  Set Printing All.
+
+
+  set (s' := update (Proj:=PC) s (offset 1 (proj (Proj:=PC) s))).
